Weidenbach_Book/IsaSAT/IsaSAT_Literals_LLVM.thy
@@ -23,6 +23,9 @@ lemma RETURN_comp_5_10_hnr_post[to_hnr_post]:
   \<open>(RETURN o\<^sub>1\<^sub>2 f12)$a$b$c$d$e$f$g$h$i$j$k$l = RETURN$(f12$a$b$c$d$e$f$g$h$i$j$k$l)\<close>
   \<open>(RETURN o\<^sub>1\<^sub>3 f13)$a$b$c$d$e$f$g$h$i$j$k$l$m = RETURN$(f13$a$b$c$d$e$f$g$h$i$j$k$l$m)\<close>
   \<open>(RETURN o\<^sub>1\<^sub>4 f14)$a$b$c$d$e$f$g$h$i$j$k$l$m$n = RETURN$(f14$a$b$c$d$e$f$g$h$i$j$k$l$m$n)\<close>
+  \<open>(RETURN o\<^sub>1\<^sub>5 f15)$a$b$c$d$e$f$g$h$i$j$k$l$m$n$xo = RETURN$(f15$a$b$c$d$e$f$g$h$i$j$k$l$m$n$xo)\<close>
+  \<open>(RETURN o\<^sub>1\<^sub>6 f16)$a$b$c$d$e$f$g$h$i$j$k$l$m$n$xo$p = RETURN$(f16$a$b$c$d$e$f$g$h$i$j$k$l$m$n$xo$p)\<close>
+  \<open>(RETURN o\<^sub>1\<^sub>7 f17)$a$b$c$d$e$f$g$h$i$j$k$l$m$n$xo$p$q = RETURN$(f17$a$b$c$d$e$f$g$h$i$j$k$l$m$n$xo$p$q)\<close>
   by simp_all
 
 method synthesize_free =
